Added extraction code, and hooked linear into the checker.

checker/builtins.ml
@@ -6,11 +6,36 @@ module C = Checker
 module MT = MTypes
 module P = Parse
 module S = Spec
+module C_impl = Checker_impl
+
+let impl_vprop_of_vprop = function
+| MT.ILe (x, k) -> C_impl.ILeq (C_impl.nat_of_int x, k)
+| MT.IEq (x, k) -> C_impl.IEq (C_impl.nat_of_int x, k)
+| MT.BTrue x -> C_impl.BTrue (C_impl.nat_of_int x)
+
+let impl_lit_of_lit = function
+| MT.Pos vp -> C_impl.Pos (impl_vprop_of_vprop vp)
+| MT.Neg vp -> C_impl.Neg (impl_vprop_of_vprop vp)
+
+let impl_clause_of_clause = List.map impl_lit_of_lit
 
 let int_list = S.listof S.intconst
 let ivar_list model = S.listof (P.parse_ivar model)
 
-let register () = ()
+let check_linear_le model =
+ fun tokens ->
+   let (coeffs, (vars, k)) =
+     (S.cons int_list (S.cons (ivar_list model) S.intconst)) tokens in
+   let linterms = List.map2 (fun c v -> (c, C_impl.nat_of_int v)) coeffs vars in
+{
+  C.repr = "linear_le" ;
+  C.check =
+    (fun cl ->
+      C_impl.check_lincon (linterms, k) (impl_clause_of_clause cl))
+}
+
+let register () =
+  R.add "linear_le" check_linear_le
 (*
   R.add "clause" R.null_checker ;
   R.add "linear_le" R.null_checker
