checker/checker_impl.v
@@ -1,0 +1,12 @@
+(* Extraction of the implemented checkers. *)
+Require Import ExtrOcamlIntConv.
+Require Import ExtrOcamlZInt.
+Require bounds.
+Require linear.
+Require cumulative.
+Require reif.
+Require element.
+
+Set Extraction Optimize.
+Extraction "checker_impl.ml" cumulative.check_cumul reif.check_reif linear.check_lincon
+  nat_of_int int_of_nat.
